\section{Matemáticas}
\subsection{Identidades}
    $C_n = \frac{2(2n-1)}{n+1} C_{n-1}$

    $C_n = \frac{1}{n+1} \binom{2n}{n}$

    $C_n \sim \frac{4^n}{n^{3/2}\sqrt{\pi}}$

    $F_{2n+1} = F_{n}^2 + F_{n+1}^2$

    $F_{2n} = F_{n+1}^2 - F_{n-1}^2$

    $\sum_{i=1}^n F_i = F_{n+2}-1$

    $F_{n+i}F_{n+j} - F_nF_{n+i+j} = (-1)^n F_iF_j$

    $\sum_{i=0}^n{r^i} = \frac{r^{n+1}-1}{r-1}$
    
    $\sum_{i=1}^n{i^2} = \frac{n\cdot(n+1)\cdot(2n+1)}{6}$

    $\sum_{i=1}^n{i^3} = \left(\frac{n\cdot(n+1)}{2}\right)^2$

    $\sum_{i=1}^n{i^4} = \frac{n\cdot(n+1)\cdot(2n+1)\cdot(3n^2+3n-1)}{12}$

    $\sum_{i=1}^{ n} i^5 = \left(\frac{ n \cdot (n+1)}{2}\right) ^2 \cdot \frac{2 n ^2 + 2n - 1}{3}$

    $\sum_{i=1}^n{\binom{n-1}{i-1}} = 2^{n-1}$

    $\sum_{i=1}^n{i\cdot\binom{n-1}{i-1}} = n\cdot2^{n-1}$

    (Möbius Inv. Formula)
    Let
    \[g(n) = \sum_{d\mid n} f(d) \texttt{, then}\]
    \[f(n)=\sum_{d\mid n} g(d) \mu\left(\frac{n}{d}\right)\]

\subsection{Convolución rápida (FFT y Karatsuba)}
\kotlinfile{fft.kt}
\kotlinfile{karatsuba.kt}

\subsection{Criba de Eratostenes}
\kotlinfile{criba_eratostenes.kt}

\subsection{Potencia binaria}
\kotlinfile{bin_pow.kt}

\subsection{Combinatoria}
\kotlinfile{combinatory.kt}